theories/Pointed.v
@@ -6,35 +6,40 @@ Require Import Overture.
 Local Open Scope path_scope.
 Local Open Scope equiv_scope.
 
-(** Allow ourselves to implicitly generalize over types [A] and [B], and a function [f]. *)
-Generalizable Variables A B f.
+(** Allow ourselves to implicitly generalize over types [A] and [B], a function [f], and a hypothesis [H]. *)
+Generalizable Variables A B f H.
 
 (** Any contratible type is pointed. *)
-Instance ispointed_contr `{Contr A} : IsPointed A := center A.
+Canonical Structure ispointed_contr `{Contr A} : IsPointed A
+  := Build_IsPointed (center A).
 
 (** A pi type with a pointed target is pointed. *)
-Instance ispointed_forall `{H : forall a : A, IsPointed (B a)}
+(** I'm not sure why I need to explicitly pass the instance to [point] here. -Jason Gross *)
+Canonical Structure ispointed_forall `{H : forall a : A, IsPointed (B a)}
 : IsPointed (forall a, B a)
-  := fun a => point (B a).
+  := Build_IsPointed (fun a => @point (B a) (H a)).
 
 (** A sigma type of pointed components is pointed. *)
-Instance ispointed_sigma `{IsPointed A} `{IsPointed (B (point A))}
+Canonical Structure ispointed_sigma A (B : A -> Type)
+          `{H : IsPointed A} `{H' : IsPointed (B (@point A H))}
 : IsPointed (sigT B)
-  := (point A; point (B (point A))).
+  := Build_IsPointed (point A; @point (B (@point A H)) H').
 
 (** A cartesian product of pointed types is pointed. *)
-Instance ispointed_prod `{IsPointed A, IsPointed B} : IsPointed (A * B)
-  := (point A, point B).
+Canonical Structure ispointed_pord `{HA : IsPointed A, HB : IsPointed B}
+: IsPointed (A * B)
+  := Build_IsPointed (@point A HA, @point B HB).
 
 (** The type [x = x] is pointed. *)
-Instance ispointed_loop_space A (a : A) : IsPointed (a = a) := idpath.
+Canonical Structure ispointed_loop_space A (a : A) : IsPointed (a = a)
+  := Build_IsPointed idpath.
 
 (** We can build an iterated loop space *)
-Definition loopSpace (A : pointedType) : pointedType :=
-  (A.1 = A.1; idpath).
+Definition loopSpace (A : pointedType) : pointedType
+  := (A.1 = A.1; Build_IsPointed idpath).
 
 Fixpoint iteratedLoopSpace (n : nat) (A : Type) `{H : IsPointed A} {struct n} : pointedType
   := match n with
-       | O => existT IsPointed A (@point A H)
-       | S p => iteratedLoopSpace p (point = point)
+       | O => existT IsPointed A H
+       | S p => @iteratedLoopSpace p (point = point) (ispointed_loop_space _ _)
      end.
